ironfleet/src/Dafny/Distributed/Concur/Movers.i.dfy
@@ -45,24 +45,8 @@ module MoversModule {
         }
         else if entry1.action.ActionEvent? && entry1.action.e.LockEvent? {
             var lock := entry1.action.e.lock;
-            ls2' := ls3.(heap := ls3.heap[ToU(lock) := ToU(NoActor())]);
-
-            assert ls2.heap[ToU(lock) := ToU(NoActor())] == ls1.heap;
-
-            if entry2.action.ActionEvent? {
-                if entry2.action.e.ReadPtrEvent? {
-                    assume ToU(lock) != ToU(entry2.action.e.ptr_read);
-                }
-                else if entry2.action.e.WritePtrEvent? {
-                    assume ToU(lock) != ToU(entry2.action.e.ptr_write);
-                }
-                else if entry2.action.e.ReadArrayEvent? {
-                    assume ToU(lock) != ToU(entry2.action.e.arr_read);
-                }
-                else if entry2.action.e.WriteArrayEvent? {
-                    assume ToU(lock) != ToU(entry2.action.e.arr_write);
-                }
-            }
+            ls2' := ls3.(locks := ls3.locks[lock := NoActor()]);
+            assert ls2.locks[lock := NoActor()] == ls1.locks;
         }
         else if entry2.action.ActionEvent? && entry2.action.e.UdpSendEvent? {
             ls2' := ls1.(sent_packets := ls1.sent_packets + {entry2.action.e.s});
@@ -72,30 +56,8 @@ module MoversModule {
         }
         else if entry2.action.ActionEvent? && entry2.action.e.UnlockEvent? {
             var lock := entry2.action.e.unlock;
-            ls2' := ls1.(heap := ls1.heap[ToU(lock) := ToU(NoActor())]);
-
-            assert ls2.heap[ToU(lock) := ToU(NoActor())] == ls3.heap;
-
-            if entry1.action.ActionEvent? {
-                if entry1.action.e.ReadPtrEvent? {
-                    assume ToU(lock) != ToU(entry1.action.e.ptr_read);
-                }
-                else if entry1.action.e.WritePtrEvent? {
-                    assume ToU(lock) != ToU(entry1.action.e.ptr_write);
-                }
-                else if entry1.action.e.ReadArrayEvent? {
-                    assume ToU(lock) != ToU(entry1.action.e.arr_read);
-                }
-                else if entry1.action.e.WriteArrayEvent? {
-                    assume ToU(lock) != ToU(entry1.action.e.arr_write);
-                }
-                else if entry1.action.e.MakePtrEvent? {
-                    assume ToU(lock) != ToU(entry1.action.e.ptr_make);
-                }
-                else if entry1.action.e.MakeArrayEvent? {
-                    assume ToU(lock) != ToU(entry1.action.e.arr_make);
-                }
-            }
+            ls2' := ls1.(locks := ls1.locks[lock := NoActor()]);
+            assert ls2.locks[lock := NoActor()] == ls3.locks;
         }
     }
 
